chore: cleanup spinlock

Iris/Iris/HeapLang/Lib/SpinLock.lean
@@ -12,41 +12,48 @@ open BI Iris ProgramLogic
 
 @[expose] public section
 
-def spinlock_newlock : Val := hl_val(λ _, ref(#false))
-def spinlock_try_acquire : Val := hl_val(λ l, snd(cmpXchg(l, #false, #true)))
-def spinlock_acquire : Val :=
-  hl_val(rec acquire l := if ({spinlock_try_acquire} l) then #() else acquire l)
-def spinlock_release : Val := hl_val(λ l, l ← #false)
+namespace SpinLock
+
+def newlock : Val := hl_val(
+  λ _, ref(#false))
+def tryAcquire : Val := hl_val(
+  λ l, snd(cmpXchg(l, #false, #true)))
+def acquire : Val := hl_val(
+  rec acquire l :=
+    if ({tryAcquire} l)
+      then #()
+      else acquire l)
+def release : Val := hl_val(
+  λ l, l ← #false)
 
 abbrev SpinLockG (GF : BundledGFunctors) := TokenG GF
 
 def spinlockN : Namespace := ndot nroot "spinlock"
 
-section SpinLockPredicates
+section Predicates
 
 variable [HeapLangGS hlc GF] [SpinLockG GF]
 
 def locked (γ : GName) : IProp GF := token γ
 
-def lock_inv (γ : GName) (l : Loc) (R : IProp GF) : IProp GF :=
-  iprop(∃ b : Bool, (l ↦ Option.some hl_val(#b)) ∗ (if b then True else locked γ ∗ R))
+def lockInv (γ : GName) (l : Loc) (R : IProp GF) : IProp GF := iprop%
+  ∃ b : Bool, (l ↦ some hl_val(#b)) ∗ (if b then True else locked γ ∗ R)
 
-def is_lock (γ : GName) (lk : Val) (R : IProp GF) : IProp GF :=
-  iprop(∃ l : Loc, ⌜lk = Val.lit (.loc l)⌝ ∧ inv spinlockN (lock_inv γ l R))
+def isLock (γ : GName) (lk : Val) (R : IProp GF) : IProp GF := iprop%
+  ∃ l : Loc, ⌜lk = Val.lit (.loc l)⌝ ∧ inv spinlockN (lockInv γ l R)
 
-instance is_lock_persistent (γ : GName) (lk : Val) (R : IProp GF) : Persistent (is_lock γ lk R) := by
-  unfold is_lock; infer_instance
+instance instIsLockPersistent (γ : GName) (lk : Val) (R : IProp GF) : Persistent (isLock γ lk R) := by
+  unfold isLock; infer_instance
 
-instance locked_timeless (γ : GName) : Timeless (locked (GF := GF) γ) := by
+instance instLockedTimeless (γ : GName) : Timeless (locked (GF := GF) γ) := by
   unfold locked; infer_instance
 
-theorem locked_exclusive (γ : GName) :
-    (locked γ ∗ locked γ) ⊢@{IProp GF} False :=
+theorem instLockedExclusive (γ : GName) : locked γ ∗ locked γ ⊢@{IProp GF} False :=
   token_exclusive γ
 
 theorem is_lock_iff (γ : GName) (lk : Val) (R₁ R₂ : IProp GF) :
-    is_lock γ lk R₁ ⊢ (▷ □ (R₁ ∗-∗ R₂)) -∗ is_lock γ lk R₂ := by
-  unfold is_lock lock_inv
+    isLock γ lk R₁ ⊢ (▷ □ (R₁ ∗-∗ R₂)) -∗ isLock γ lk R₂ := by
+  unfold isLock lockInv
   iintro ⟨%l, %H1, #H2⟩ #Heq
   iexists l
   isplit; itrivial
@@ -64,64 +71,62 @@ theorem is_lock_iff (γ : GName) (lk : Val) (R₁ R₂ : IProp GF) :
     icases H3 with ⟨$, H3⟩
     iapply Heq $$ H3
 
-end SpinLockPredicates
+end Predicates
 
-section SpinLockSpecs
+section Specs
 
 variable {GF : BundledGFunctors} [HeapLangGS hlc GF] [SpinLockG GF]
 
-theorem spinlock_newlock_spec :
+theorem newlock_spec :
   ⊢ □ ∀ (Φ : Val → IProp GF),
-    (∀ (v : Val) (γ : GName), (∀ R E, R ={E}=∗ is_lock γ v R) -∗ Φ v)
-    -∗ WP hl({spinlock_newlock} #()) {{ Φ }} := by
-  unfold spinlock_newlock
-  imodintro
-  iintro %Φ Hcont
+    (∀ (v : Val) (γ : GName), (∀ R E, R ={E}=∗ isLock γ v R) -∗ Φ v) -∗
+    WP hl({newlock} #()) {{ Φ }} := by
+  unfold newlock
+  iintro !> %Φ Hcont
   iapply wp_rec; simp only [Exp.subst]
   inext
   imod token_alloc with ⟨%γ, Hγ⟩
-  iapply wp_wand (Φ := fun v => iprop(∃ l', ⌜v = hl_val(#(BaseLit.loc l'))⌝ ∗ l' ↦ some hl_val(#false)))
-  · iapply wp_alloc
+  iapply wp_wand; iapply wp_alloc
   iintro %v ⟨%l, %Heq, Hpt⟩
   iapply Hcont $$ %v %γ
   iintro %R %E HR
-  imod inv_alloc spinlockN E iprop(∃ b, (l ↦ some hl_val(#(BaseLit.bool b))) ∗ if b = true then True else token γ ∗ R) $$ [Hpt HR Hγ]
+  ihave HI : ▷ ∃ b, (l ↦ some hl_val(#(BaseLit.bool b))) ∗ if b = true then True else token γ ∗ R $$
+      [Hpt HR Hγ]
   · iexists false
     simp only [Bool.false_eq_true, ↓reduceIte]
     iframe
-  · subst Heq
-    imodintro
-    unfold is_lock
-    iexists l
-    isplit; itrivial
-    unfold lock_inv locked
-    iframe
-
-theorem spinlock_try_acquire_spec (γ : GName) (lk : Val) (R : IProp GF) :
-    ⊢ □ ∀ (Φ : Val → IProp GF),
-    is_lock γ lk R
-    -∗ (∀ (b : Bool), iprop(if b then locked γ ∗ R else iprop(True)) -∗ Φ hl_val(#b))
-    -∗ WP hl({spinlock_try_acquire} {lk}) {{ Φ }} := by
-  unfold spinlock_try_acquire
+  imod inv_alloc spinlockN E _ $$ HI with H
   imodintro
-  iintro %Φ #Hlock Hcont
+  unfold isLock
+  iexists l
+  subst Heq
+  isplit; itrivial
+  unfold lockInv locked
+  iframe
+
+theorem try_acquire_spec (γ : GName) (lk : Val) (R : IProp GF) :
+    ⊢ □ ∀ (Φ : Val → IProp GF),
+    isLock γ lk R -∗
+    (∀ (b : Bool), iprop(if b then locked γ ∗ R else iprop(True)) -∗ Φ hl_val(#b)) -∗
+    WP hl({tryAcquire} {lk}) {{ Φ }} := by
+  unfold tryAcquire
+  iintro !> %Φ #Hlock Hcont
   iapply wp_rec; simp only [Exp.subst, Exp.substStr, BEq.rfl, ↓reduceIte]
   inext
-  unfold is_lock
+  unfold isLock
   icases Hlock with ⟨%l, %Heq, #Hinv⟩
   subst Heq
   iapply wp_bind (fun x => hl(snd({x})))
   iapply wp_atomic (E2 := ⊤ \ nclose spinlockN)
   imod inv_acc ⊤ _ _ (fun _ _ => CoPset.mem_full) $$ Hinv with ⟨G1, G2⟩
-  unfold lock_inv
+  unfold lockInv
   imodintro
   icases G1 with ⟨%b, Hpt, Hcond⟩
   cases b
   · simp only [Bool.false_eq_true, ↓reduceIte]
     iapply wp_wand $$ [Hpt]
-    · iapply wp_cmpXchg_true (by rfl) (by rfl) $$ Hpt
-      · simp [Val.compareSafe, Val.isUnboxed, BaseLit.isUnboxed]
-      · trivial
+    · iapply wp_cmpXchg_true rfl rfl $$ Hpt <;>
+        simp [Val.compareSafe, Val.isUnboxed, BaseLit.isUnboxed]
     iintro %v ⟨%Heq, Hpt⟩
     subst Heq
     imod G2 $$ [Hpt]
@@ -136,9 +141,8 @@ theorem spinlock_try_acquire_spec (γ : GName) (lk : Val) (R : IProp GF) :
       iframe
   · simp only [↓reduceIte]
     iapply wp_wand $$ [Hpt]
-    · iapply wp_cmpXchg_fail (by rfl) (by rfl) $$ Hpt
-      · simp [Val.compareSafe, Val.isUnboxed, BaseLit.isUnboxed]
-      · simp
+    · iapply wp_cmpXchg_fail rfl rfl $$ Hpt <;>
+        simp [Val.compareSafe, Val.isUnboxed, BaseLit.isUnboxed]
     iintro %v ⟨%Heq, Hpt⟩
     subst Heq
     imod G2 $$ [Hpt]
@@ -151,19 +155,19 @@ theorem spinlock_try_acquire_spec (γ : GName) (lk : Val) (R : IProp GF) :
       simp only [Bool.false_eq_true, ↓reduceIte]
       itrivial
 
-theorem spinlock_acquire_spec (γ : GName) (lk : Val) (R : IProp GF) :
+theorem acquire_spec (γ : GName) (lk : Val) (R : IProp GF) :
   ⊢ □ ∀ (Φ : Val → IProp GF),
-    is_lock γ lk R
-    -∗ (locked γ ∗ R -∗ Φ hl_val(#()))
-    -∗ WP hl({spinlock_acquire} {lk}) {{ Φ }} := by
-  unfold spinlock_acquire
+    isLock γ lk R -∗
+    (locked γ ∗ R -∗ Φ hl_val(#())) -∗
+    WP hl({acquire} {lk}) {{ Φ }} := by
+  unfold acquire
   iintro !> %Φ #Hlock Hcont
   iloeb as IH
-  iapply wp_rec; simp only [Exp.subst, Exp.substStr, String.reduceBEq, Bool.false_eq_true,
-    ↓reduceIte, BEq.rfl]
+  iapply wp_rec
+  simp only [Exp.subst, Exp.substStr, String.reduceBEq, Bool.false_eq_true, ↓reduceIte, BEq.rfl]
   inext
   iapply wp_bind (fun x => hl(if {x} then {?_} else {?_})) (κ := instContextExpValStateObservationIf)
-  iapply spinlock_try_acquire_spec $$ Hlock
+  iapply try_acquire_spec $$ Hlock
   iintro %b Hpt
   cases b
   · iapply wp_if_false
@@ -177,21 +181,21 @@ theorem spinlock_acquire_spec (γ : GName) (lk : Val) (R : IProp GF) :
     simp only [if_pos]
     iframe
 
-theorem spinlock_release_spec (γ : GName) (lk : Val) (R : IProp GF) :
+theorem release_spec (γ : GName) (lk : Val) (R : IProp GF) :
   ⊢ □ ∀ (Φ : Val → IProp GF),
-    is_lock γ lk R ∗ (locked γ ∗ R)
-    -∗ (True -∗ Φ hl_val(#()))
-    -∗ WP hl({spinlock_release} {lk}) {{ Φ }} := by
-  unfold spinlock_release
+    isLock γ lk R ∗ (locked γ ∗ R) -∗
+    (True -∗ Φ hl_val(#())) -∗
+    WP hl({release} {lk}) {{ Φ }} := by
+  unfold release
   iintro !> %Φ ⟨#Hlock, ⟨Hl, HR⟩⟩ Hcont
   iapply wp_rec; simp only [Exp.subst, Exp.substStr, ↓reduceIte, BEq.rfl]
   inext
-  unfold is_lock
+  unfold isLock
   icases Hlock with ⟨%l, %Heq, #Hinv⟩
   subst Heq
   iapply wp_atomic (E2 := ⊤ \ nclose spinlockN)
   imod inv_acc ⊤ _ _ (fun _ _ => CoPset.mem_full) $$ Hinv with ⟨G1, G2⟩
-  unfold lock_inv
+  unfold lockInv
   imodintro
   icases G1 with ⟨%b, Hpt, Hcond⟩
   iapply wp_wand $$ [Hpt]
@@ -208,23 +212,24 @@ theorem spinlock_release_spec (γ : GName) (lk : Val) (R : IProp GF) :
     iapply Hcont
     itrivial
 
-end SpinLockSpecs
+end Specs
 
 @[implicit_reducible]
-def spinLock [HeapLangGS hlc GF] : Lock GF where
-  newlock := spinlock_newlock
-  acquire := spinlock_acquire
-  release := spinlock_release
+def instLock [HeapLangGS hlc GF] : Lock GF where
+  newlock := newlock
+  acquire := acquire
+  release := release
   lockG   := SpinLockG
   name := GName
-  isLock _ γ lk R  := is_lock γ lk R
+  isLock _ γ lk R  := isLock γ lk R
   locked _ γ := locked γ
-  isLock_persistent γ lk R := is_lock_persistent γ lk R
+  isLock_persistent γ lk R := instIsLockPersistent γ lk R
   isLock_iff γ lk R₁ R₂ := is_lock_iff γ lk R₁ R₂
-  locked_timeless γ := locked_timeless γ
-  locked_exclusive γ := locked_exclusive γ
-  newlock_spec_delay_init := spinlock_newlock_spec
-  acquire_spec γ lk R := spinlock_acquire_spec γ lk R
-  release_spec γ lk R := spinlock_release_spec γ lk R
+  locked_timeless γ := instLockedTimeless γ
+  locked_exclusive γ := instLockedExclusive γ
+  newlock_spec_delay_init := newlock_spec
+  acquire_spec γ lk R := acquire_spec γ lk R
+  release_spec γ lk R := release_spec γ lk R
 
+end SpinLock
 end
